coq: Add the multiplier correctness proofs

examples/rv/Multiplier.v
@@ -1,8 +1,8 @@
 (*! Implementation of a multiplier module !*)
 Require Import Coq.Lists.List.
 
-Require Import Koika.Frontend.
-Require Import Koika.Std.
+Require Import Koika.Frontend Koika.Std Koika.SemanticProperties Koika.Common.
+Require Import Lia.
 
 Module Type Multiplier_sig.
   Parameter n: nat.
@@ -85,3 +85,410 @@ Module Multiplier (s: Multiplier_sig).
   Instance FiniteType_reg_t : FiniteType reg_t := _.
 
 End Multiplier.
+
+Module MultiplierProofs.
+  Module Sig32 <: Multiplier_sig.
+    Definition n := 32.
+  End Sig32.
+  Module mul32 := Multiplier Sig32.
+  Import mul32.
+  Import Sig32.
+
+  Notation n := 32.
+
+  Definition default := ContextEnv.(create) r.
+
+  Definition typed_enq :=
+    tc_function R empty_Sigma enq.
+
+  Definition typed_step :=
+    tc_function R empty_Sigma step.
+
+  Definition typed_deq :=
+    tc_function R empty_Sigma deq.
+
+  Notation all_regs :=
+    [valid; operand1; operand2; result; n_step; finished].
+
+  Ltac simpl_interp_hypothesis :=
+    repeat match goal with
+           | _ => progress (simpl cassoc in *; simpl ctl in *; simpl chd in *)
+           | [ H: match ?x with | Some(_) => _ | None => None end = Some (_) |- _ ] =>
+             destruct x eqn:?; [ | solve [inversion H] ]
+           | [ H: (if ?x then _ else None) = Some _ |- _ ] =>
+             destruct x eqn:?; [ | solve [inversion H] ]
+           | _ => progress cleanup_log_step
+           end.
+
+  Ltac simpl_interp_action :=
+    match goal with
+    | [ H: interp_action _ _ _ _ _ ?action = Some _ |- _] =>
+      unfold action in H;
+      simpl (projT2 _) in H;
+      unfold interp_action in H;
+      unfold opt_bind in H;
+      unfold no_latest_writes in *;
+      repeat cleanup_log_step
+    end.
+
+  Ltac simpl_interp_action_all :=
+    simpl_interp_action;
+    repeat match goal with
+           | _ => progress simpl_interp_hypothesis
+           | [ H: (if ?c then _ else _) = Some (_, _, _) |- _ ] =>
+             destruct c eqn:?
+           end.
+
+  (* This might require another hypothesis to be correct *)
+  Lemma sel_spec :
+    forall (sz: nat) (bs: bits sz) idx,
+      BitFuns.sel bs idx = Ob~(N.testbit (Bits.to_N bs) (Bits.to_N idx)).
+  Proof.
+  Admitted.
+
+  Lemma to_N_lsl :
+    forall sz1 sz2 (x: bits sz1) (y: bits sz2),
+      (Bits.to_N (BitFuns.lsl x y) =
+       (Bits.to_N x * (2 ^ (Bits.to_N y))) mod (2 ^ N.of_nat sz1))%N.
+  Proof.
+  Admitted.
+
+  Lemma to_N_extend_end_false :
+    forall sz (x: bits sz) sz', Bits.to_N (Bits.extend_end x sz' false) = Bits.to_N x.
+  Proof.
+  Admitted.
+
+  Ltac Bits_to_N_t :=
+    unfold PrimSpecs.sigma1, CircuitPrimSpecs.sigma1,
+    PrimSpecs.sigma2, CircuitPrimSpecs.sigma2,
+    Bits.plus, Bits.mul in *;
+    simpl arg1Sig;
+    repeat match goal with
+           | _ => progress bool_step
+           | _ => progress (rewrite Bits.of_N_to_N in * )
+           | [ H: Ob~_ = Ob~_ |- _ ] => injection H as H
+           | [ H: Bits.single (Bits.neg _) = true |- _ ] =>
+             apply negb_true_iff in H
+           | [ H: Bits.single (Bits.neg _) = false |- _ ] =>
+             apply negb_false_iff in H
+           | [ H: Bits.single (Bits.and _ _) = true |- _ ] =>
+             apply andb_true_iff in H; destruct H
+           | [ H: Bits.single (Bits.and _ _) = false |- _ ] =>
+             apply andb_false_iff in H
+           | [ H: Bits.single (BitFuns._eq _ _) = true |- _ ] =>
+             apply beq_dec_iff in H
+           | [ H: Bits.single (BitFuns._eq _ _) = false |- _ ] =>
+             apply beq_dec_false_iff in H
+           | [ H: Bits.single ?bs = _ |- _ ] =>
+             apply Bits.single_to_bits in H
+           | _ => progress (rewrite sel_spec in *)
+           | [ H: context[Bits.to_N (BitFuns.lsl ?x ?y)] |- _ ] =>
+             rewrite to_N_lsl in H
+           | [ |- context[Bits.to_N (BitFuns.lsl ?x ?y)] ] =>
+             rewrite to_N_lsl
+           | [ H: context[Bits.to_N (Bits.extend_end ?bs ?sz' false)] |- _ ] =>
+             setoid_rewrite (to_N_extend_end_false (Bits.size bs) bs sz') in H
+           | [ |- context[Bits.to_N (Bits.extend_end ?bs ?sz' false)] ] =>
+             setoid_rewrite (to_N_extend_end_false (Bits.size bs) bs sz')
+           | [ H: _ = _ |- _ ] =>
+             apply (f_equal Bits.to_N) in H
+           | [ H: _ <> _ |- _ ] =>
+             apply Bits.to_N_inj_contra in H
+           end.
+
+  Ltac remember_bits_to_N_ n :=
+    match goal with
+    | [ H: n = ?x |- _ ] =>
+      is_var x
+    | _ =>
+      let Hx := fresh "H" in
+      remember n eqn:Hx;
+      symmetry in Hx;
+      setoid_rewrite_in_all Hx
+    end.
+
+  Ltac remember_bits_to_N :=
+    repeat match goal with
+           | [ |- context[Bits.to_N ?bs] ] =>
+             progress (remember_bits_to_N_ (Bits.to_N bs))
+           | [ H: context[Bits.to_N ?bs] |- _ ] =>
+             progress (remember_bits_to_N_ (Bits.to_N bs))
+           end.
+
+  Ltac pose_bits_bound_proofs :=
+    repeat match goal with
+           | [ H: context[Bits.to_N ?bs] |- _ ] =>
+             let sz := eval hnf in (Bits.size bs) in
+             pose_once Bits.to_N_bounded sz bs
+           | [ |- context[Bits.to_N ?bs] ] =>
+             let sz := eval hnf in (Bits.size bs) in
+             pose_once Bits.to_N_bounded sz bs
+           end.
+
+  Ltac lia_bits :=
+    cbn in *; pose_bits_bound_proofs; remember_bits_to_N; cbn in *; lia.
+
+  Definition partial_mul (a b n_step: N) :=
+    (a * (b mod (2 ^ n_step)))%N.
+
+  Lemma partial_mul_step (a b n_step: N) :
+    partial_mul a b (n_step + 1) =
+    ((partial_mul a b n_step) +
+     a * (N.b2n (N.testbit b n_step) * (2 ^ n_step)))%N.
+  Proof.
+  Admitted.
+
+  Definition step_invariant (reg: ContextEnv.(env_t) R) :=
+    (Bits.to_N (ContextEnv.(getenv) reg n_step) < N.of_nat n)%N.
+
+  Definition finished_invariant (reg: ContextEnv.(env_t) R) :=
+    let valid_val := Bits.to_N (ContextEnv.(getenv) reg valid) in
+    let finished_val := Bits.to_N (ContextEnv.(getenv) reg finished) in
+    valid_val = 0%N -> finished_val = 0%N.
+
+  Definition result_invariant (reg: ContextEnv.(env_t) R) :=
+    let valid_val := Bits.to_N (ContextEnv.(getenv) reg valid) in
+    let finished_val := Bits.to_N (ContextEnv.(getenv) reg finished) in
+    let result_val := Bits.to_N (ContextEnv.(getenv) reg result) in
+    let op1_val := Bits.to_N (ContextEnv.(getenv) reg operand1) in
+    let op2_val := Bits.to_N (ContextEnv.(getenv) reg operand2) in
+    let n_step_val := Bits.to_N (ContextEnv.(getenv) reg n_step) in
+    valid_val = 1%N ->
+    finished_val = 0%N ->
+    result_val = partial_mul op1_val op2_val n_step_val.
+
+  Definition result_finished_invariant (reg: ContextEnv.(env_t) R) :=
+    let finished_val := Bits.to_N (ContextEnv.(getenv) reg finished) in
+    let result_val := Bits.to_N (ContextEnv.(getenv) reg result) in
+    let op1_val := Bits.to_N (ContextEnv.(getenv) reg operand1) in
+    let op2_val := Bits.to_N (ContextEnv.(getenv) reg operand2) in
+    finished_val = 1%N ->
+    (result_val = op1_val * op2_val)%N.
+
+  Definition invariant reg :=
+    step_invariant reg /\
+    finished_invariant reg /\
+    result_invariant reg /\
+    result_finished_invariant reg.
+
+  Lemma enq_preserves_invariant :
+    forall env Gamma sched_log action_log action_log_new v Gamma_new,
+      invariant (commit_update env sched_log) ->
+      no_latest_writes action_log all_regs ->
+      interp_action env empty_sigma Gamma sched_log action_log typed_enq =
+      Some (action_log_new, v, Gamma_new) ->
+      invariant (commit_update env (log_app action_log_new sched_log)).
+  Proof.
+    intros.
+    unfold invariant, step_invariant, finished_invariant,
+           result_invariant, result_finished_invariant in *.
+    simpl_interp_action_all.
+    Bits_to_N_t.
+    repeat (split).
+    - discriminate.
+    - intros.
+      unfold partial_mul. cbn.
+      rewrite N.mod_1_r.
+      ring.
+    - intros.
+      match goal with
+      | [ H1: ?x = ?y, H2: _ -> ?x = ?z |- _ ] =>
+        rewrite H2 in H1; [ discriminate | auto ]
+      end.
+  Qed.
+
+  Lemma deq_preserves_invariant :
+    forall env Gamma sched_log action_log action_log_new v Gamma_new,
+      invariant (commit_update env sched_log) ->
+      no_latest_writes action_log all_regs ->
+      interp_action env empty_sigma Gamma sched_log action_log typed_deq =
+      Some (action_log_new, v, Gamma_new) ->
+      invariant (commit_update env (log_app action_log_new sched_log)).
+  Proof.
+    intros.
+    unfold invariant, step_invariant, finished_invariant, result_invariant in *.
+    simpl_interp_action_all.
+    Bits_to_N_t.
+    repeat (split); auto || discriminate.
+  Qed.
+
+  Lemma step_preserves_finished_invariant :
+    forall env Gamma sched_log action_log action_log_new v Gamma_new,
+      invariant (commit_update env sched_log) ->
+      no_latest_writes action_log all_regs ->
+      interp_action env empty_sigma Gamma sched_log action_log typed_step =
+      Some (action_log_new, v, Gamma_new) ->
+      finished_invariant (commit_update env (log_app action_log_new sched_log)).
+  Proof.
+    intros.
+    unfold invariant, step_invariant, finished_invariant, result_invariant in *.
+    simpl_interp_action_all;
+    Bits_to_N_t;
+    intros;
+    match goal with
+    | [H1: ?x = ?y, H2: ?x = ?z |- _ ] => rewrite H1 in H2; discriminate H2
+    end.
+  Qed.
+
+  Lemma step_preserves_step_invariant :
+    forall env Gamma sched_log action_log action_log_new v Gamma_new,
+      invariant (commit_update env sched_log) ->
+      no_latest_writes action_log all_regs ->
+      interp_action env empty_sigma Gamma sched_log action_log typed_step =
+      Some (action_log_new, v, Gamma_new) ->
+      step_invariant (commit_update env (log_app action_log_new sched_log)).
+  Proof.
+    intros.
+    unfold invariant, step_invariant, finished_invariant, result_invariant in *.
+    simpl_interp_action_all;
+    Bits_to_N_t; try (assumption);
+    rewrite Bits.to_N_of_N;
+    lia_bits.
+  Qed.
+
+  (* The admitted subgoals should be handle by lia_bits *)
+  Lemma step_preserves_result_invariant :
+    forall env Gamma sched_log action_log action_log_new v Gamma_new,
+      invariant (commit_update env sched_log) ->
+      no_latest_writes action_log all_regs ->
+      no_latest_writes sched_log all_regs ->
+      interp_action env empty_sigma Gamma sched_log action_log typed_step =
+      Some (action_log_new, v, Gamma_new) ->
+      result_invariant (commit_update env (log_app action_log_new sched_log)).
+  Proof.
+    intros.
+    unfold invariant, step_invariant, finished_invariant, result_invariant in *.
+    simpl_interp_action_all;
+    intros;
+    Bits_to_N_t;
+    unfold Sig32.n in *;
+    try discriminate.
+    match goal with
+    | [ H: context[_ = partial_mul _ _ _] |- _ ] =>
+      setoid_rewrite H; try assumption
+    end; cbn in *.
+    - rewrite Bits.to_N_of_N.
+      + rewrite Bits.to_N_of_N; [ | lia_bits ].
+        cbn. rewrite_all_hypotheses. cbn.
+        rewrite partial_mul_step.
+        rewrite_all_hypotheses.
+        f_equal. cbn [N.b2n].
+        admit.
+      + admit.
+    - rewrite Bits.to_N_of_N; [ | lia_bits ].
+      rewrite partial_mul_step.
+      rewrite_all_hypotheses. cbn.
+      rewrite N.mul_0_r. rewrite N.add_0_r.
+      auto.
+  Admitted.
+
+  Lemma mul_to_partial_mul :
+    forall n x y,
+      (y < 2 ^ n)%N ->
+      (x * y = partial_mul x y n)%N.
+  Proof.
+    intros.
+    unfold partial_mul.
+    rewrite N.mod_small; auto.
+  Qed.
+
+  Lemma step_preserves_result_finished_invariant :
+    forall env Gamma sched_log action_log action_log_new v Gamma_new,
+      invariant (commit_update env sched_log) ->
+      no_latest_writes action_log all_regs ->
+      no_latest_writes sched_log all_regs ->
+      interp_action env empty_sigma Gamma sched_log action_log typed_step =
+      Some (action_log_new, v, Gamma_new) ->
+      result_finished_invariant (commit_update env (log_app action_log_new sched_log)).
+  Proof.
+    intros.
+    unfold invariant, step_invariant, finished_invariant, result_invariant, result_finished_invariant in *.
+    simpl_interp_action_all;
+    intros;
+    Bits_to_N_t;
+    unfold Sig32.n in *;
+    try match goal with
+        | [ H1: ?x = ?y, H2: ?x = ?z |- _ ] =>
+          rewrite H1 in H2; discriminate H2
+        end;
+    match goal with
+    | [ H: context[_ = partial_mul _ _ _] |- _ ] =>
+      setoid_rewrite H; try assumption
+    end;
+    cbn in *.
+    - rewrite_all_hypotheses.
+      rewrite Bits.to_N_of_N.
+      + rewrite N.mod_small; [ | lia_bits ].
+        rewrite (mul_to_partial_mul (N.of_nat Sig32.n) (Bits.to_N _) (Bits.to_N _)); [ | lia_bits ].
+        cbn.
+        assert (32 = 31 + 1)%N as H32S by reflexivity.
+        rewrite H32S.
+        rewrite partial_mul_step.
+        repeat (f_equal; []).
+        match goal with
+        | [ H1: ?x = ?y, H2: context[N.testbit _ _] |- _ ] =>
+          rewrite H1 in H2
+        end.
+        rewrite_all_hypotheses.
+        reflexivity.
+      + admit.
+    - rewrite_all_hypotheses.
+      rewrite (mul_to_partial_mul (N.of_nat Sig32.n)); [ | lia_bits ].
+      cbn.
+      assert (32 = 31 + 1)%N as H32S by reflexivity.
+      rewrite H32S.
+      rewrite partial_mul_step.
+      repeat (f_equal; []).
+      match goal with
+      | [ H1: ?x = ?y, H2: context[N.testbit _ _] |- _ ] =>
+        rewrite H1 in H2
+      end.
+      rewrite_all_hypotheses. cbn.
+      rewrite N.mul_0_r. rewrite N.add_0_r.
+      reflexivity.
+    Admitted.
+
+  Lemma enq_set_operands :
+    forall (env: ContextEnv.(env_t) R) Gamma sched_log action_log action_log_new v Gamma_new,
+      no_latest_writes action_log [operand1; operand2] ->
+      interp_action env empty_sigma Gamma sched_log action_log typed_enq =
+      Some (action_log_new, v, Gamma_new) ->
+      latest_write action_log_new operand1 = Some (chd Gamma) /\
+      latest_write action_log_new operand2 = Some (chd (ctl Gamma)).
+  Proof.
+    intros.
+    simpl_interp_action_all.
+    auto.
+  Qed.
+
+  Lemma step_keep_operands :
+    forall (env: ContextEnv.(env_t) R) Gamma sched_log action_log action_log_new v Gamma_new,
+      no_latest_writes action_log [operand1; operand2] ->
+      interp_action env empty_sigma Gamma sched_log action_log typed_step =
+      Some (action_log_new, v, Gamma_new) ->
+      no_latest_writes action_log_new [operand1; operand2].
+  Proof.
+    intros.
+    simpl_interp_action_all;
+    auto.
+  Qed.
+
+  Lemma deq_result :
+    forall env Gamma sched_log action_log action_log_new v Gamma_new,
+      invariant (commit_update env sched_log) ->
+      no_latest_writes action_log all_regs ->
+      no_latest_writes sched_log all_regs ->
+      interp_action env empty_sigma Gamma sched_log action_log typed_deq =
+      Some (action_log_new, v, Gamma_new) ->
+      let operand1_val := Bits.to_N (ContextEnv.(getenv) env operand1) in
+      let operand2_val := Bits.to_N (ContextEnv.(getenv) env operand2) in
+      (Bits.to_N v = operand1_val * operand2_val)%N.
+  Proof.
+    intros.
+    unfold invariant, result_finished_invariant in *.
+    simpl_interp_action_all.
+    Bits_to_N_t.
+    auto.
+  Qed.
+
+End MultiplierProofs.
